Rename ConstRef to ConstRefFunc.

WebAssembly/Wasm.thy
@@ -107,7 +107,7 @@ inductive b_e_typing :: "[t_context, b_e list, tf] \<Rightarrow> bool" ("_ \<tur
 
 inductive ref_typing :: "[s, v_ref, t_ref] => bool" where
    "ref_typing s (ConstNull t) (t)"
- | "f < length (funcs s) \<Longrightarrow> ref_typing s (ConstRef f) (T_func_ref)"
+ | "f < length (funcs s) \<Longrightarrow> ref_typing s (ConstRefFunc f) (T_func_ref)"
  | "ref_typing s (ConstRefExtern _) (T_ext_ref)"
 
 inductive v_typing :: "s \<Rightarrow> v \<Rightarrow> t \<Rightarrow> bool" where
@@ -298,14 +298,14 @@ inductive reduce :: "[s, f, e list, s, f, e list] \<Rightarrow> bool" ("\<lparr>
   \<comment> \<open>\<open>call\<close>\<close>
 | call:"\<lparr>s;f;[$(Call j)]\<rparr> \<leadsto> \<lparr>s;f;[Invoke (sfunc_ind (f_inst f) j)]\<rparr>"
   \<comment> \<open>\<open>call_indirect\<close>\<close>
-| call_indirect_Some:"\<lbrakk>(f_inst f) = i; stab s i ti (nat_of_int c) = Some (ConstRef i_cl); stypes i j = tf; cl_type (funcs s!i_cl) = tf\<rbrakk> \<Longrightarrow> \<lparr>s;f;[$EConstNum (ConstInt32 c), $(Call_indirect ti j)]\<rparr> \<leadsto> \<lparr>s;f;[Invoke i_cl]\<rparr>"
-| call_indirect_None:"\<lbrakk>(f_inst f) = i; (stab s i ti (nat_of_int c) = Some (ConstRef i_cl) \<and> stypes i j \<noteq> cl_type (funcs s!i_cl)) \<or> \<not> is_some_const_ref_func (stab s i ti (nat_of_int c))\<rbrakk> \<Longrightarrow> \<lparr>s;f;[$EConstNum (ConstInt32 c), $(Call_indirect ti j)]\<rparr> \<leadsto> \<lparr>s;f;[Trap]\<rparr>"
+| call_indirect_Some:"\<lbrakk>(f_inst f) = i; stab s i ti (nat_of_int c) = Some (ConstRefFunc i_cl); stypes i j = tf; cl_type (funcs s!i_cl) = tf\<rbrakk> \<Longrightarrow> \<lparr>s;f;[$EConstNum (ConstInt32 c), $(Call_indirect ti j)]\<rparr> \<leadsto> \<lparr>s;f;[Invoke i_cl]\<rparr>"
+| call_indirect_None:"\<lbrakk>(f_inst f) = i; (stab s i ti (nat_of_int c) = Some (ConstRefFunc i_cl) \<and> stypes i j \<noteq> cl_type (funcs s!i_cl)) \<or> \<not> is_some_const_ref_func (stab s i ti (nat_of_int c))\<rbrakk> \<Longrightarrow> \<lparr>s;f;[$EConstNum (ConstInt32 c), $(Call_indirect ti j)]\<rparr> \<leadsto> \<lparr>s;f;[Trap]\<rparr>"
   \<comment> \<open>\<open>invoke\<close>\<close>
 | invoke_native:"\<lbrakk>(funcs s!i_cl) = Func_native j (t1s _> t2s) ts es; ves = ($C* vcs); length vcs = n; length ts = k; length t1s = n; length t2s = m; (n_zeros ts = Some zs) \<rbrakk> \<Longrightarrow> \<lparr>s;f;ves @ [Invoke i_cl]\<rparr> \<leadsto> \<lparr>s;f;[Frame m \<lparr> f_locs = vcs@zs, f_inst = j \<rparr> [(Label m [] ($*es))]]\<rparr>"
 | invoke_host_Some:"\<lbrakk>(funcs s!i_cl) = Func_host (t1s _> t2s) h; ves = ($C* vcs); length vcs = n; length t1s = n; length t2s = m; host_apply s (t1s _> t2s) h vcs hs (Some (s', vcs'))\<rbrakk> \<Longrightarrow> \<lparr>s;f;ves @ [Invoke i_cl]\<rparr> \<leadsto> \<lparr>s';f;($C* vcs')\<rparr>"
 | invoke_host_None:"\<lbrakk>(funcs s!i_cl) = Func_host (t1s _> t2s) h; ves = ($C* vcs); length vcs = n; length t1s = n; length t2s = m\<rbrakk> \<Longrightarrow> \<lparr>s;f;ves @ [Invoke i_cl]\<rparr> \<leadsto> \<lparr>s;f;[Trap]\<rparr>"
   \<comment> \<open>\<open>references\<close>\<close>
-| func_ref: "\<lbrakk>length fi = j; (inst.funcs (f_inst f)) = (fi @ [fa] @ fas)\<rbrakk> \<Longrightarrow> \<lparr>s;f;[$(Func_ref j)]\<rparr> \<leadsto> \<lparr>s;f;[Ref (ConstRef (fa))]\<rparr>"
+| func_ref: "\<lbrakk>length fi = j; (inst.funcs (f_inst f)) = (fi @ [fa] @ fas)\<rbrakk> \<Longrightarrow> \<lparr>s;f;[$(Func_ref j)]\<rparr> \<leadsto> \<lparr>s;f;[Ref (ConstRefFunc (fa))]\<rparr>"
   \<comment> \<open>\<open>get_local\<close>\<close>
 | get_local:"\<lbrakk>length vi = j; f_locs f = (vi @ [v] @ vs)\<rbrakk> \<Longrightarrow> \<lparr>s;f;[$(Get_local j)]\<rparr> \<leadsto> \<lparr>s;f;[$C v]\<rparr>"
   \<comment> \<open>\<open>set_local\<close>\<close>
